src/3d/Ast.fst
@@ -533,7 +533,6 @@ type decl' =
   | OutputType : out_typ -> decl'
   | ExternType : typedef_names -> decl'
   | ExternFn   : ident -> typ -> list param -> decl'
-  | CompileTimeFlag : ident -> decl'  
 
 [@@ PpxDerivingYoJson ]
 noeq
@@ -754,8 +753,7 @@ let subst_decl' (s:subst) (d:decl') : ML decl' =
     CaseType names (subst_params s params) (subst_switch_case s cases)
   | OutputType _
   | ExternType _
-  | ExternFn _ _ _
-  | CompileTimeFlag _ -> d
+  | ExternFn _ _ _ -> d
 let subst_decl (s:subst) (d:decl) : ML decl = decl_with_v d (subst_decl' s d.d_decl.v)
 
 (*** Printing the source AST; for debugging only **)
@@ -1022,7 +1020,6 @@ let print_decl' (d:decl') : ML string =
   | OutputType out_t -> "Printing for output types is TBD"
   | ExternType _ -> "Printing for extern types is TBD"
   | ExternFn _ _ _ -> "Printing for extern functions is TBD"
-  | CompileTimeFlag i -> Printf.sprintf "[@@IfDef]val %s : bool" i.v.name
 
 let print_decl (d:decl) : ML string =
   match d.d_decl.comments with
