src/3d/Config.fst
@@ -1,5 +1,5 @@
 module Config
-
+module O = Options
 [@@ PpxDerivingYoJson]
 type compile_time_flags = {
   flags : list string;
@@ -10,3 +10,12 @@ type compile_time_flags = {
 type config = {
   compile_time_flags : compile_time_flags
 }
+
+let emit_config_as_fstar_module (module_name:string) (c:config) = 
+  let flags = 
+    List.map 
+      (Printf.sprintf "[@@ CIfDef]\nassume\nval ___%s : bool" )
+      c.compile_time_flags.flags
+  in
+  let assumes = String.concat "\n\n" flags in
+  Printf.sprintf "module %s\n%s\n" module_name assumes
