src/3d/Deps.fsti
@@ -23,4 +23,4 @@ val has_extern_types (g:dep_graph) (modul:string) : bool
 
 val has_extern_functions (g:dep_graph) (modul:string) : bool
 
-val get_config (_:unit) : ML (option Config.config)
+val get_config (_:unit) : ML (option (Config.config & string))
